theories/Factor_Finite_Program_History_Inspection.thy
@@ -1,0 +1,99 @@
+theory Factor_Finite_Program_History_Inspection
+  imports Factor_Finite_Program_Histories
+begin
+
+definition finite_program_history_steps where
+  "finite_program_history_steps P D A Hs=(
+    iteration_prefix (\<lambda>X. finite_inference_next (finite_program_rule_table P D) {||} X\<noteq>X)
+      (finite_inference_next (finite_program_rule_table P D) {||}) {||} (map fst Hs) A \<and>
+    finite_inference_next (finite_program_rule_table P D) {||} A=A)"
+
+definition program_history_steps where
+  "program_history_steps P D A Hs=(
+    iteration_prefix (\<lambda>X. finite_inference_round (finite_program_rule_table P D) {||} X\<noteq>X)
+      (finite_inference_round (finite_program_rule_table P D) {||}) {}
+      (map (\<lambda>(X,W). fset X) Hs) (fset A) \<and>
+    finite_inference_round (finite_program_rule_table P D) {||} (fset A)=fset A)"
+
+lemma finite_program_history_steps_exact:
+  "finite_program_history_steps P D A Hs=program_history_steps P D A Hs"
+proof -
+  have injective: "inj fset" by (simp add: inj_on_def fset_inject)
+  have path: "iteration_prefix
+      (\<lambda>X. finite_inference_round (finite_program_rule_table P D) {||} X\<noteq>X)
+      (finite_inference_round (finite_program_rule_table P D) {||}) (fset {||})
+      (map fset (map fst Hs)) (fset A) \<longleftrightarrow>
+    iteration_prefix
+      (\<lambda>X. finite_inference_next (finite_program_rule_table P D) {||} X\<noteq>X)
+      (finite_inference_next (finite_program_rule_table P D) {||}) {||} (map fst Hs) A"
+    by (rule iteration_prefix_map[OF injective])
+      (rule finite_inference_next_test, rule finite_inference_next_correct)
+  show ?thesis
+    using path by (simp add: finite_program_history_steps_def program_history_steps_def
+      finite_inference_next_fixed comp_def split_def)
+qed
+
+definition finite_program_history_witnesses where
+  "finite_program_history_witnesses P D Hs=
+    list_all (\<lambda>(X,W). W=finite_program_activation P D X) Hs"
+
+definition program_history_witnesses where
+  "program_history_witnesses P D Hs=(\<forall>(X,W)\<in>set Hs. \<forall>d c t V H.
+    (d,c,t,V,H) |\<in>| W \<longleftrightarrow>
+      (d,t) |\<in>| D \<and>
+      admitted_schema_instance (decode_finite_system P) d c (decode_finite_term_bindings V)
+        (decode_finite_term t) (decode_finite_premises H) \<and>
+      fimage snd H |\<subseteq>| X)"
+
+lemma finite_program_history_witnesses_exact:
+  assumes "finite_program_head_covered P D"
+  shows "finite_program_history_witnesses P D Hs=program_history_witnesses P D Hs"
+proof -
+  have each: "W=finite_program_activation P D X \<longleftrightarrow>
+      (\<forall>d c t V H. (d,c,t,V,H) |\<in>| W \<longleftrightarrow> (d,t) |\<in>| D \<and>
+        admitted_schema_instance (decode_finite_system P) d c (decode_finite_term_bindings V)
+          (decode_finite_term t) (decode_finite_premises H) \<and> fimage snd H |\<subseteq>| X)" for X W
+    by (simp only: fset_eq_iff split_paired_All finite_program_activation_exact[OF assms])
+  show ?thesis
+    by (auto simp only: finite_program_history_witnesses_def program_history_witnesses_def
+      list_all_iff each split: prod.splits)
+qed
+
+theorem finite_program_history_inspection:
+  assumes result: "finite_program_history P D=Some (A,Hs)"
+  shows "finite_program_history_steps P D A Hs"
+    "finite_program_history_witnesses P D Hs"
+proof -
+  obtain Xs where history: "finite_inference_history (finite_program_rule_table P D) {||}=Some (A,Xs)"
+    and labels: "Hs=map (\<lambda>X. (X,finite_program_activation P D X)) Xs"
+    using result by (simp only: finite_program_history_conditions; blast)
+  show "finite_program_history_steps P D A Hs"
+    using finite_inference_history_correct(2,3)[OF history]
+    by (simp add: finite_program_history_steps_def labels comp_def)
+  show "finite_program_history_witnesses P D Hs"
+    by (simp add: finite_program_history_witnesses_def labels list_all_iff)
+qed
+
+definition finite_program_history_step_review where
+  "finite_program_history_step_review P D A Hs=
+    iteration_review (\<lambda>X. finite_inference_next (finite_program_rule_table P D) {||} X\<noteq>X)
+      (finite_inference_next (finite_program_rule_table P D) {||}) {||} (map fst Hs) A"
+
+lemma finite_program_history_step_review_exact:
+  "iteration_review_holds (finite_program_history_step_review P D A Hs)=finite_program_history_steps P D A Hs"
+  by (simp add: finite_program_history_step_review_def iteration_review_exact finite_program_history_steps_def)
+
+definition finite_program_history_witness_review where
+  "finite_program_history_witness_review P D Hs=
+    finite_inference_witness_review finite_program_application_rule (finite_program_applications P D) Hs"
+
+lemma finite_program_history_witness_review_exact:
+  "finite_inference_witness_review_holds (finite_program_history_witness_review P D Hs)=
+    finite_program_history_witnesses P D Hs"
+  by (simp only: finite_program_history_witness_review_def finite_inference_witness_review_exact
+    finite_program_history_witnesses_def finite_program_activation_def)
+
+export_code finite_program_history_steps finite_program_history_witnesses
+  finite_program_history_step_review finite_program_history_witness_review checking SML
+
+end
