theories/Finite_Set_Transformations.thy
@@ -1,0 +1,19 @@
+theory Finite_Set_Transformations
+  imports "HOL-Library.FSet"
+begin
+
+lemma finite_image_restriction:
+  assumes "B |\<subseteq>| fimage f A"
+  shows "fimage f (ffilter (\<lambda>x. f x |\<in>| B) A)=B"
+  by (rule fset_inject[THEN iffD1])
+    (use assms in \<open>auto simp: less_eq_fset.rep_eq fimage.rep_eq\<close>)
+
+lemma finite_difference_empty:
+  "A |-| B={||} \<longleftrightarrow> A |\<subseteq>| B"
+  by (auto simp: fset_eq_iff less_eq_fset.rep_eq)
+
+lemma finite_differences_empty:
+  "A |-| B={||} \<and> B |-| A={||} \<longleftrightarrow> A=B"
+  by (auto simp: finite_difference_empty intro: order_antisym)
+
+end
